concurrency/verif_bst_flows.v
@@ -1,0 +1,268 @@
+Require Import bst.puretree.
+Require Import VST.floyd.proofauto.
+Require Import VST.progs.bst.
+Require Import VST.msl.iter_sepcon.
+Require Import bst.flows.
+Require Import bst.val_countable.
+Require Import bst.inset_flows.
+Require Import bst.verif_bst_flows_safe.
+Require Import bst.sepalg_ext.
+
+Open Scope Z_scope.
+Open Scope logic.
+
+Definition bst_inset_flowint := inset_flowint TreeNode Z.
+
+Definition inset_global_inv (root: TreeNode) (NS: list TreeNode)
+           (Iset: bst_inset_flowint) : Prop :=
+  keyset_global_inv root Iset /\ list_to_set (map key_tn NS) ⊆ KS.
+
+Definition gmap_sub `{Countable K} {A} (s1 s2: gmap K A): Prop :=
+  forall k a, s1 !! k = Some a -> s2 !! k = Some a.
+
+Lemma nzmap_subset_wf: forall `{Countable K} `{CCM A} (s1 s2: gmap K A),
+    gmap_sub s1 s2 -> nzmap_wf s2 -> nzmap_wf s1.
+Proof.
+  unfold nzmap_wf. intros. rewrite map_Forall_lookup in H2 |- *. intros.
+  rewrite map_Forall_lookup. intros. apply (H2 i). now apply H1.
+Qed.
+
+Lemma split_filter_sub: forall {K A} `{Countable K} (m: gmap K A) f,
+    gmap_sub (list_to_map (List.filter f (map_to_list m))) m.
+Proof.
+  intros. unfold gmap_sub. intros. apply elem_of_list_to_map_2 in H0.
+  apply elem_of_list_In in H0. apply filter_In in H0. destruct H0.
+  rewrite <- elem_of_map_to_list. now rewrite elem_of_list_In.
+Qed.
+
+Definition splitLeft (mulst: gmap Z nat) (e: Z): gmap Z nat :=
+  list_to_map (List.filter (fun zn => (fst zn) <? e) (map_to_list mulst)).
+
+Lemma nzmap_left_wf: forall m e,  nzmap_wf m -> nzmap_wf (splitLeft m e).
+Proof. intros. apply nzmap_subset_wf with m; auto. apply split_filter_sub. Qed.
+
+Definition splitRight (mulst: gmap Z nat) (e: Z): gmap Z nat :=
+  list_to_map (List.filter (fun zn => (fst zn) >? e) (map_to_list mulst)).
+
+Lemma nzmap_right_wf: forall m e,  nzmap_wf m -> nzmap_wf (splitRight m e).
+Proof. intros. apply nzmap_subset_wf with m; auto. apply split_filter_sub. Qed.
+
+Definition split_left (s: K_multiset Z) (e: Z): K_multiset Z :=
+  let (m, Hm) := s in
+  NZMap (splitLeft m e)
+        (bool_decide_pack _ (nzmap_left_wf m e (bool_decide_unpack _ Hm))).
+
+Definition split_right (s: K_multiset Z) (e: Z): K_multiset Z :=
+  let (m, Hm) := s in
+  NZMap (splitRight m e)
+        (bool_decide_pack _ (nzmap_right_wf m e (bool_decide_unpack _ Hm))).
+
+Definition inset_edgeFn (x y: TreeNode): K_multiset Z -> K_multiset Z :=
+  fun s => if (val_eqb x.(addr_tn) y.(addr_tn) || val_eqb y.(addr_tn) nullval)%bool
+           then ∅
+           else if val_eqb y.(addr_tn) x.(left_tn)
+                then split_left s x.(key_tn)
+                else if val_eqb y.(addr_tn) x.(right_tn)
+                     then split_right s x.(key_tn)
+                     else ∅.
+
+Definition inset_local_inv (t: TreeNode) (It: bst_inset_flowint): Prop :=
+  ✓ It /\ domm It = {[t]} /\ in_inset t.(key_tn) It t /\
+  (forall n, out It n = inset_edgeFn t n (inf It t)).
+
+Definition node_rep (t: TreeNode) (Ipc: pc_flowint) (Is: bst_inset_flowint): mpred :=
+  !! (inset_local_inv t Is /\ pc_local_inv t Ipc) &&
+  data_at Tsh t_struct_tree (Vint (Int.repr t.(key_tn)),
+                             (t.(value_tn), (t.(left_tn), t.(right_tn)))) t.(addr_tn).
+
+Definition tree_rep (l: list TreeNode) (Cpc: pc_flowint)
+           (Cs: bst_inset_flowint): mpred :=
+  EX fpc fs, !! (list_join fpc Cpc /\ list_join fs Cs /\
+                  Datatypes.length fpc = Datatypes.length l /\
+                  Datatypes.length fs = Datatypes.length l) &&
+              iter_sepcon (fun x => node_rep x.1 x.2.1 x.2.2)
+                          (combine l (combine fpc fs)).
+
+Definition treebox_rep root l Cpc Cs (b: val) :=
+  !!(pc_global_inv root l Cpc /\ inset_global_inv root l Cs) &&
+  data_at Tsh (tptr t_struct_tree) (addr_tn root) b * tree_rep l Cpc Cs.
+
+Definition lookup_spec :=
+ DECLARE _lookup
+  WITH b: val, x: Z, v: val, root: TreeNode, l: (list TreeNode), Cpc: pc_flowint,
+       Cs: bst_inset_flowint
+  PRE [ tptr (tptr t_struct_tree), tint  ]
+    PROP (Int.min_signed <= x <= Int.max_signed; x ∈ KS)
+    PARAMS(b; Vint (Int.repr x))
+    SEP (treebox_rep root l Cpc Cs b)
+  POST [ tptr Tvoid ]
+    EX r,
+    PROP ((~ In x (map key_tn l) /\ r = nullval) \/
+          (exists t, In t l /\ key_tn t = x /\ value_tn t = r))
+    RETURN (r)
+    SEP (treebox_rep root l Cpc Cs b).
+
+Definition Gprog : funspecs := ltac:(with_library prog [lookup_spec]).
+
+Lemma tree_rep_impl_pc_tree_rep: forall l C C', tree_rep l C C' |-- pc_tree_rep l C.
+Proof.
+  intros. unfold tree_rep, pc_tree_rep. Intros fpc fs. Exists fpc. entailer.
+  apply derives_trans with
+      (iter_sepcon
+         (λ x : TreeNode * (pc_flowint * bst_inset_flowint), pc_node_rep x.1 x.2.1)
+         (combine l (combine fpc fs))).
+  - apply conclib.iter_sepcon_derives. intros. destruct x as [t [Ipc Is]]. simpl.
+    unfold node_rep, pc_node_rep. entailer !.
+  - revert fpc fs C C' H1 H2 H H0. induction l; intros; simpl; auto.
+    destruct fpc as [|Ipc fpc]. 1: simpl in H1; lia.
+    destruct fs as [|Is fs]. 1: simpl in H2; lia. simpl. cancel. inv H. inv H0.
+    eapply IHl; eauto.
+Qed.
+
+Lemma tree_rep_has_children: forall root l C C',
+    !!(pc_global_inv root l C) && tree_rep l C C' |--
+             !!(forall x, In x l ->
+                          has_child_or_none x left_tn l /\
+                          has_child_or_none x right_tn l).
+Proof.
+  intros. apply derives_trans with (!!(pc_global_inv root l C) && pc_tree_rep l C).
+  - Intros. entailer !. apply tree_rep_impl_pc_tree_rep.
+  - apply pc_tree_rep_has_children.
+Qed.
+
+Lemma tree_rep_is_ptr_null: forall n l C1 C2,
+    In n l -> tree_rep l C1 C2 |-- !! is_pointer_or_null (addr_tn n).
+Proof.
+  intros. apply derives_trans with (pc_tree_rep l C1).
+  - apply tree_rep_impl_pc_tree_rep.
+  - now apply pc_tree_rep_is_ptr_null.
+Qed.
+
+Lemma tree_rep_saturate_local: forall root l C C',
+    pc_global_inv root l C -> tree_rep l C C' |--
+                                          !! is_pointer_or_null (addr_tn root).
+Proof.
+  intros. apply derives_trans with (pc_tree_rep l C).
+  - apply tree_rep_impl_pc_tree_rep.
+  - now apply pc_tree_rep_saturate_local.
+Qed.
+
+Lemma tree_rep_neq_nullval: forall n l C1 C2,
+    In n l -> tree_rep l C1 C2 |-- !! (addr_tn n <> nullval).
+Proof.
+  intros. apply derives_trans with (pc_tree_rep l C1).
+  - apply tree_rep_impl_pc_tree_rep.
+  - rewrite (pc_tree_rep_In_eq n); auto. Intros nI l' Cl.
+    unfold pc_node_rep. Intros. entailer !.
+Qed.
+
+Lemma tree_rep_cons: forall n l C1 C2,
+    tree_rep (n :: l) C1 C2 =
+    EX nI nS Cl1 Cl2, !! (intJoin nI Cl1 C1 /\ intJoin nS Cl2 C2) &&
+                      node_rep n nI nS * tree_rep l Cl1 Cl2.
+Proof.
+  intros. apply pred_ext.
+  - unfold tree_rep. Intros fpc fs. destruct fpc. 1: simpl in H1; lia.
+    destruct fs. 1: simpl in H2; lia. inv H. inv H0.
+    simpl. Exists p b lj lj0. entailer!. Exists fpc fs. entailer !.
+  - Intros nI nS Cl1 Cl2. unfold tree_rep. Intros fpc fs.
+    Exists (nI :: fpc) (nS :: fs). simpl. entailer!.
+    split; econstructor; eauto.
+Qed.
+
+Lemma tree_rep_perm': forall l1 l2 C1 C2,
+    Permutation l1 l2 -> tree_rep l1 C1 C2 |-- tree_rep l2 C1 C2.
+Proof.
+  intros. revert C1 C2. induction H; auto; intros.
+  - rewrite !tree_rep_cons. Intros nI nS Cl1 Cl2. Exists nI nS Cl1 Cl2. entailer !.
+  - rewrite tree_rep_cons. Intros nIy nSy Cl1y Cl2y. do 2 rewrite tree_rep_cons.
+    Intros nIx nSx Cl1x Cl2x. Exists nIx nSx. apply intJoin_comm in H, H0.
+    destruct (intJoin_assoc _ _ _ _ _ H1 H) as [xyI []]. Exists xyI.
+    destruct (intJoin_assoc _ _ _ _ _ H2 H0) as [xyS []]. Exists xyS. entailer !.
+    rewrite tree_rep_cons. Exists nIy nSy Cl1x Cl2x. apply intJoin_comm in H3, H5.
+    entailer !.
+  - now transitivity (tree_rep l' C1 C2).
+Qed.
+
+Lemma tree_rep_perm: forall l1 l2 C1 C2,
+    Permutation l1 l2 -> tree_rep l1 C1 C2 = tree_rep l2 C1 C2.
+Proof. intros. apply pred_ext; apply tree_rep_perm'; auto. now symmetry. Qed.
+
+Lemma tree_rep_In_eq: forall n l C1 C2,
+    In n l -> tree_rep l C1 C2 =
+              EX nI nS l' Cl1 Cl2, !! (intJoin nI Cl1 C1 /\ intJoin nS Cl2 C2 /\
+                                       Permutation (n :: l') l) &&
+                                   (node_rep n nI nS * tree_rep l' Cl1 Cl2).
+Proof.
+  intros. apply pred_ext.
+  - apply in_split in H. destruct H as [l1 [l2 ?]]. subst l.
+    pose proof (Permutation_middle l1 l2 n).
+    rewrite <- (tree_rep_perm (n :: l1 ++ l2)); auto. rewrite tree_rep_cons.
+    Intros nI nS Cl1 Cl2. Exists nI nS (l1 ++ l2) Cl1 Cl2. entailer !.
+  - Intros nI nS l' Cl1 Cl2. rewrite <- (tree_rep_perm (n :: l') l); auto.
+    rewrite tree_rep_cons. Exists nI nS Cl1 Cl2. entailer !.
+Qed.
+
+Lemma node_rep_valid_ptr: forall n nI nS,
+    node_rep n nI nS |-- valid_pointer (addr_tn n).
+Proof. intros. unfold node_rep. entailer !. Qed.
+
+Definition lookup_inv (root: TreeNode) (b: val) (l: list TreeNode)
+           (Cpc : pc_flowint) (Cs: bst_inset_flowint) (x: Z): environ -> mpred :=
+  EX n: TreeNode, EX l': list TreeNode, EX nI: pc_flowint, EX Cl: pc_flowint,
+  EX nS: bst_inset_flowint, EX Cls: bst_inset_flowint,
+    PROP (intJoin nI Cl Cpc; intJoin nS Cls Cs; in_inset x nS n;
+         if Val.eq (addr_tn n) nullval
+         then nI = ∅ /\ nS = ∅ /\ l' = l /\ Cl = Cpc /\ Cls = Cs
+         else Permutation (n :: l') l)
+    LOCAL (temp _p (addr_tn n); temp _t b; temp _x (Vint (Int.repr x)))
+    SEP (data_at Tsh (tptr t_struct_tree) (addr_tn root) b;
+        if Val.eq (addr_tn n) nullval then emp else node_rep n nI nS;
+        tree_rep l' Cl Cls).
+
+Lemma body_lookup: semax_body Vprog Gprog f_lookup lookup_spec.
+Proof.
+  start_function.
+  unfold treebox_rep. Intros. sep_apply (tree_rep_has_children root l Cpc Cs); auto.
+  Intros. forward.
+  - entailer. sep_apply (tree_rep_saturate_local root l Cpc Cs); auto. entailer !.
+  - forward_while (lookup_inv root b l Cpc Cs x).
+    + Exists root. destruct H1 as [_ [_ [_ [? _]]]].
+      sep_apply (tree_rep_neq_nullval root l Cpc Cs). Intros.
+      rewrite (tree_rep_In_eq root l Cpc Cs H1). Intros nI nS l' Cl1 Cl2.
+      Exists l' nI Cl1 nS Cl2. if_tac. 1: now exfalso.
+      assert_PROP (root ∈ domm nS). {
+        unfold node_rep. Intros. apply prop_right. destruct H9 as [_ [? _]].
+        rewrite H9. now apply elem_of_singleton_2. } entailer !.
+      destruct H2 as [[? [_ [_ ?]]] _]. eapply inset_monotone; eauto.
+    + if_tac.
+      * Intros. subst. rewrite H4. entailer !.
+      * sep_apply node_rep_valid_ptr. Intros. entailer !.
+    + if_tac. 1: now exfalso. unfold node_rep. Intros.
+      assert (In n l). {
+        eapply Permutation_in; eauto. now left. }
+      assert (data_at Tsh t_struct_tree
+                      (Vint (Int.repr (key_tn n)),
+                       (value_tn n, (left_tn n, right_tn n))) (addr_tn n) *
+              tree_rep l' Cl Cls |-- tree_rep l Cpc Cs). {
+        rewrite (tree_rep_In_eq n l Cpc Cs); auto. Exists nI nS l' Cl Cls.
+        unfold node_rep. entailer !. } forward. specialize (H3 _ H11).
+      destruct H3. forward_if.
+      * forward; sep_apply H12; destruct H3 as [? | [p [? [? ?]]]].
+        -- rewrite H3. entailer !.
+        -- rewrite H16. sep_apply (tree_rep_is_ptr_null p l Cpc Cs). entailer !.
+        -- admit.
+        -- admit.
+      * forward_if.
+        -- forward; sep_apply H12; destruct H13 as [? | [p [? [? ?]]]].
+           ++ rewrite H13; entailer !.
+           ++ rewrite H17. sep_apply (tree_rep_is_ptr_null p l Cpc Cs). entailer !.
+           ++ admit.
+           ++ admit.
+        -- forward; destruct H10 as [? [? [? [? [? [? [? ?]]]]]]].
+           ++ entailer !.
+           ++ sep_apply H12. forward. Exists (value_tn n). unfold treebox_rep.
+              entailer !. right. exists n. split; [|split]; auto.
+              rewrite Int.signed_repr in H14, H15; auto. lia.
+    + if_tac. 2: now exfalso.
+Abort.
